Cslib/Computability/Machines/MultiTapeTuring/Satisfiability.lean
@@ -180,8 +180,7 @@ public def sat_verify : MultiTapeTM 5 Char :=
 public theorem sat_verify.computes_fun
   {views : Fin 5 → TapeView}
   (h_input : (views 0).current = some (StrEnc.toData (SATInput.mk formula assignments)))
-  (h_second_empty : views 1 = TapeView.empty)
-  (h_third_empty_list : views 2 = TapeView.ofList []) :
+  (h_second_empty : views 1 = TapeView.empty) :
    sat_verify.eval_struct views = some (Function.update views 2
      ((views 2).pushList (StrEnc.toData (evalFormula assignments formula)))) := by
   let line₁ : MultiTapeTM 5 Char := toElem 1 0 ;ₜ copyEnc 0 1 (by decide) ;ₜ outOfList 0
@@ -199,10 +198,21 @@ public theorem sat_verify.computes_fun
       outOfList_eval_struct_valid, line₂]
     rw [sat_verify_core_semantics _ (by simp [TapeView.current_rev, h_v1]) (by simp [h_v2])]
     simp [h_v1, h_v2, TapeView.current_rev, Function.update_sort]
-  -- simp [sat_verify, line₁, h_line₁, line₂, h_line₂, h_input]
-  -- rw [sat_verify_core_semantics _ (by sorry) (by sorry)]
-  -- simp [TapeView.current_rev]
-  sorry
+  -- Main composition
+  have h_pre₁ : (Function.update views 1 (TapeView.ofEnc assignments) 0).current =
+      some (StrEnc.toData (SATInput.mk formula assignments)) := by
+    simp [h_input]
+  have h_pre₂ : Function.update views 1 (TapeView.ofEnc assignments) 1 =
+      TapeView.ofEnc assignments := by simp
+  have h₂ := h_line₂ _ h_pre₁ h_pre₂
+  unfold sat_verify
+  change (line₁ ;ₜ toElem 0 0 ;ₜ sat_verify_core ;ₜ outOfList 0 ;ₜ erase 1).eval_struct views = _
+  simp only [seq_eval_struct, h_line₁, Option.bind_some]
+  rw [← seq_eval_struct, ← seq_eval_struct, h₂]
+  simp only [Option.bind_some, erase_eval_struct]
+  simp [Function.update_sort]
+  grind
+
 
 
 end Satisfiability
